no admits in proofs!

basic_types.v
@@ -70,6 +70,7 @@ prove_equiv_compat.
 Qed.
 
 
+
 Ltac weaken H := eapply tr_formation_weaken; apply H.
 Ltac var_solv0 := try (apply tr_hyp_tm; repeat constructor).
 
@@ -462,6 +463,12 @@ Lemma leq_succ_equiv n1_pred n2 : equiv (leq_t (ppair bfalse n1_pred) n2) (bite 
                                                              (app (ppi2 n2) triv))).
   Admitted. 
 Lemma leq_zero_equiv n2: equiv (leq_t nzero n2) unittp. Admitted.
+
+Lemma leq_succsucc_equiv n1_pred n2_pred : equiv (leq_t (ppair bfalse n1_pred)
+                                            (ppair bfalse n2_pred))                                                                               (leq_t (app n1_pred triv)
+                                                             (app n2_pred triv)).
+  Admitted. 
+
 
 Lemma leqb_succ_equiv n1_pred n2 : equiv (leqb_app (ppair bfalse n1_pred) n2) (bite (if_z n2)
                                                      bfalse
@@ -1959,3 +1966,49 @@ Lemma eqb_P G n m : tr G (oof n nattp) ->
 Qed.
 
 (*write out subseq refl and subseq trans on paper*)
+
+Definition nsucc_leq_fn :=
+    (app (app (app nat_ind_fn (lam
+                          (leq_t (var 0) (nsucc (var 0))))
+               )
+               triv )
+               (lam (*x : nat*) (lam (*IH: P(x) *)
+                                         (var 0) (*s x  <= s nsucc x  : nat*)
+                                      )
+                  )
+               ).
+
+ 
+Lemma nsucc_leq: forall G n, tr G (oof n nattp) ->
+                       tr G (oof (app nsucc_leq_fn n) (leq_t n (nsucc n))).
+  intros. unfold nsucc_leq_fn.
+  replace (leq_t n (nsucc n)) with (subst1 n (leq_t (var 0) (nsucc (var 0)))).
+  2:{ simpsub_big. auto. } apply (tr_pi_elim _ nattp).
+    eapply nat_ind_lamapp; simpsub_big; try reflexivity.
+    { (*type p*)
+      apply tr_arrow_intro; try apply leq_type; try apply nsucc_type; try var_solv'; auto. }
+    { eapply tr_compute; try apply leq_zero_equiv; try apply equiv_refl. constructor.
+    }
+    {
+      apply tr_pi_intro; auto. apply tr_arrow_intro; try weaken leq_type.
+      var_solv'.
+      apply nsucc_type; var_solv'. 
+      apply nsucc_type; var_solv'.
+      repeat apply nsucc_type; var_solv'.
+      simpsub. eapply tr_compute. 
+      eapply equiv_trans.
+      { try apply leq_succsucc_equiv; try apply equiv_refl. }
+      { apply equiv_app. apply equiv_app. apply equiv_refl.
+        apply reduce_equiv. apply reduce_app_beta; apply reduce_id. 
+        apply reduce_equiv. apply reduce_app_beta; apply reduce_id. 
+      }
+      apply equiv_refl. apply equiv_refl.
+      simpsub. simpl. 
+      change 
+       (app (app leqtp (var 1))
+            (nsucc (var 1))) with (subst sh1
+          (leq_t (var 0)
+             (nsucc (var 0)))
+                                  ). var_solv0.
+    } assumption.
+Qed.
