basic_types_working.v
@@ -5,383 +5,53 @@ From istari Require Import Sigma Tactics
      Syntax Subst SimpSub Promote Hygiene
      ContextHygiene Equivalence Equivalences Rules Defined PageType lemmas0 derived_rules basic_types.
 
-      Definition eqb_sound_fn :=
+Definition nsucc_leq_fn :=
     (app (app (app nat_ind_fn (lam
-                  (pi nattp
-                      ( (*x = 1, y = 0*)
-                        arrow 
-                        (equal booltp (app (eq_b (var 1)) (var 0)) btrue
-                               )
-                        (equal nattp (var 1) (var 0))
-                  )
-               )))
-               (lam (*y : nat*)
-                  (lam  (*hyp : eqb 0 y  = tt*)
-                  triv 
-                  )
-               ))
-               (lam (*x : nat*) (lam (*IH: P(x) ie pi y (eqb x y = t -> x = y)*)
-                                   (lam  (*y'  : nat*)
-                                      (lam (*eqb s x y' = t*)
-                                         triv (*s x  = y  : nat*)
+                          (leq_t (var 0) (nsucc (var 0))))
+               )
+               triv )
+               (lam (*x : nat*) (lam (*IH: P(x) *)
+                                         (var 0) (*s x  <= s nsucc x  : nat*)
                                       )
                   )
-               ))).
-     (*          
-  tr
-    [:: hyp_tm
-          (equal booltp
-             (if_z (var 0)) btrue),
-        hyp_tm nattp
-      & G]
-    (deq nzero
-       (var (1 + 0)%coq_nat) nattp) *)
+               ).
 
-      Lemma bool_contra G J : tr G (deq bfalse btrue booltp) ->
-                          tr G J.
-    Admitted.
+Lemma leq_succsucc_equiv n1_pred n2_pred : equiv (leq_t (ppair bfalse n1_pred)
+                                            (ppair bfalse n2_pred))                                                                               (leq_t (app n1_pred triv)
+                                                             (app n2_pred triv)).
+  Admitted. 
 
-      Lemma equal_nzero_help G n:
-        tr G (oof n nattp) -> tr G (oof (lam triv)
-                                       (arrow (equal booltp (if_z n) btrue)
-                                              (equal nattp nzero n)
-                                       )
-                                  ).
-        intros. 
-        replace 
-    (oof (lam triv)
-       (arrow
-          (equal booltp 
-             (if_z n) btrue)
-          (equal nattp nzero n)))
- with
-            (substj (dot n id) 
-    (oof (lam triv)
-       (arrow
-          (equal booltp 
-             (if_z (var 0)) btrue)
-          (equal nattp nzero (var 0))))) .
-        2:{ simpl. simpsub_big. auto. } 
-        eapply (tr_generalize _ nattp). assumption.
-        apply tr_arrow_intro; auto. { apply tr_equal_formation; auto.
-                                      weaken tr_booltp_formation.
-                                      apply if_z_typed. var_solv'. constructor. }
-                                    { apply tr_equal_formation; auto. var_solv'. }
-                                    simpsub_big.
-        rewrite make_app1. eapply w_elim_hyp.
-        weaken tr_booltp_formation. weaken nat_U01.
-        change triv with (@subst obj (under 1 (dot (ppi2 (var 0)) (dot (ppi1 (var 0)) sh1))) triv). apply tr_sigma_eta_hyp. simpsub_big.
-        simpl. simpsub_big. simpl.
-        rewrite make_app2.
-      match goal with |- tr ?G (deq triv triv ?T) =>
-                      suffices: (tr G (oof (bite (var 2) triv triv) T)) end.
-      { intros Hannoying. constructor. eapply deq_intro. apply Hannoying. }
-      rewrite make_app2.
-        change triv with 
-            (@subst obj (under 2 sh1) triv).
-        apply tr_booltp_eta_hyp; simpl; simpsub_big; simpl.
-        { (*true*)
-          rewrite make_app1.
-          eapply tr_compute_hyp.
-        {
-          constructor. apply equiv_arrow. apply reduce_equiv.
-          apply reduce_bite_beta1. apply reduce_id.
-          apply equiv_refl.
-        }
-        constructor. apply tr_wt_intro. constructor.
-        simpsub_big.
-        eapply tr_compute. { apply equiv_arrow. apply reduce_equiv.
-          apply reduce_bite_beta1. apply reduce_id.
-          apply equiv_refl.
- } apply equiv_refl. apply equiv_refl.
-        apply (tr_transitivity _#2 (lam (app (subst sh1 (var 1)) (var 0)))).
-        { apply tr_arrow_intro; auto. weaken tr_voidtp_formation.
-          eapply (tr_voidtp_elim  _ (var 0) (var 0)).
-          change voidtp with (@subst obj (sh 1) voidtp). var_solv0.
-        }
-        { apply tr_symmetry. apply tr_arrow_eta.
-          change (arrow voidtp nattp) with (@subst obj (sh 2) (arrow voidtp nattp)).
-          var_solv0.
-        }
-        weaken nat_U01. }
-        {(*false*)
-          eapply (tr_compute_hyp _ [::]).
-        {
-          constructor. apply equiv_equal. apply equiv_refl. apply reduce_equiv.
-          apply reduce_ppi1_beta. apply reduce_id.
-          apply equiv_refl.
-        }
-        apply bool_contra. simpl. apply (deq_intro _#4 (var 0) (var 0)).
-        change (equal booltp bfalse btrue) with (@subst obj sh1 (equal booltp bfalse btrue)).
-        var_solv0. } 
-       Qed. 
-
-
-      Lemma equal_nzero G n:
-        tr G (oof n nattp) ->
-        tr G (deq (if_z n) btrue booltp) ->
-        tr G (deq nzero n nattp).
-        intros.
-        apply (deq_intro _#4 (app (lam triv) triv) (app (lam triv) triv)).
-        apply (tr_arrow_elim _ (equal booltp (if_z n) btrue)).
-        apply tr_equal_formation; auto. weaken tr_booltp_formation.
-        apply if_z_typed. assumption. constructor.
-        apply tr_equal_formation; auto. apply equal_nzero_help. assumption.
-        constructor. assumption. Qed.
-
-  Lemma equal_succ G preds: tr G (oof preds (arrow unittp nattp)) ->
-                        tr G (deq (nsucc (app preds triv )) (ppair bfalse preds) nattp).
-    intros. unfold nsucc. simpsub. apply tr_wt_intro. constructor.
-    simpsub_big.
-    eapply tr_compute. { apply equiv_arrow. apply reduce_equiv.
-                         apply reduce_bite_beta2. apply reduce_id. apply equiv_refl. } apply equiv_refl. apply equiv_refl.
-    apply (tr_transitivity _ _ (lam (app (subst sh1 preds) (var 0)))).
-    {
-            apply tr_arrow_intro; auto.
-            apply (tr_arrow_elim _ unittp); auto.
-            match goal with |- tr ?G (deq ?M ?M ?T) =>
-                                                      change T with
-       (@shift obj 1
-               (arrow unittp nattp)) end. rewrite subst_sh_shift. apply tr_weakening_append1.
-            assumption.
-          apply tr_symmetry. apply tr_unittp_eta.
-          change unittp with (@subst obj (sh 1) unittp). var_solv0.
-    }
-    {
-      apply tr_symmetry. apply tr_arrow_eta. assumption.
-    }
-    weaken nat_U01. Qed.
-
-  Lemma eqb_sound G : tr G (oof eqb_sound_fn (pi nattp (pi nattp (arrow (equal booltp (app (eq_b (var 1)) (var 0))
-                                                                               btrue
-                                                                        )
-                                                                        (equal nattp (var 1) (var 0))
-
-                           )))).
-    unfold eqb_sound_fn.
-    assert (forall G' x, tr G' (oof x nattp) ->
-                    tr G' (oof (pi nattp (arrow (equal booltp (app (eq_b (subst sh1 x)) (var 0))
-                                                                               btrue
-                                                                        )
-                                                                        (equal nattp (subst sh1 x) (var 0))
-
-
-                               ))
-                               U0)
-           ) as Hp.
-    {
-      intros. 
-      apply tr_pi_formation_univ; auto.
-      apply tr_arrow_formation_univ; auto.
-      apply tr_equal_formation_univ; auto.
-      simpsub_big. apply tr_booltp_formation.
-      apply eqapp_typed; try var_solv'.  change nattp with (@subst obj sh1 nattp).
-      rewrite ! subst_sh_shift. apply tr_weakening_append1. assumption.
-      constructor.
-      apply tr_equal_formation_univ; auto; try var_solv'.
-      change nattp with (@subst obj sh1 nattp).
-      rewrite ! subst_sh_shift. apply tr_weakening_append1. assumption.
-    }
+ 
+Lemma nsucc_leq: forall G n, tr G (oof n nattp) ->
+                       tr G (oof (app nsucc_leq_fn n) (leq_t n (nsucc n))).
+  intros. unfold nsucc_leq_fn.
+  replace (leq_t n (nsucc n)) with (subst1 n (leq_t (var 0) (nsucc (var 0)))).
+  2:{ simpsub_big. auto. } apply (tr_pi_elim _ nattp).
     eapply nat_ind_lamapp; simpsub_big; try reflexivity.
     { (*type p*)
-      apply tr_arrow_intro; auto. simpsub_big.
-      change (var 1) with (@subst obj sh1 (var 0)). apply Hp; var_solv'. }
-    { (*type BC*)
-       apply tr_pi_intro; auto. 
-       apply tr_arrow_intro; auto. 
-      apply tr_equal_formation; auto.
-      weaken tr_booltp_formation.
-      apply eqapp_typed; auto; try var_solv'. constructor.
-      apply tr_equal_formation; auto; try var_solv'.
-      eapply (tr_compute_hyp _ [::]). constructor. apply equiv_equal. apply equiv_refl.
-      apply eq_b0. apply equiv_refl. simpl. simpsub_big.
-      constructor. apply equal_nzero.  
-      apply (deq_intro _#4 (var 0) (var 0)). 
-      match goal with |- tr ?G (deq ?M ?M ?T) => replace T with
-          (subst sh1
-       (equal booltp
-              (if_z (var 0)) btrue)) end.
-      2:{
-        simpl. simpsub_big. auto.
-      }
-      var_solv0.
+      apply tr_arrow_intro; try apply leq_type; try apply nsucc_type; try var_solv'; auto. }
+    { eapply tr_compute; try apply leq_zero_equiv; try apply equiv_refl. constructor.
     }
-    { (*type IS*)
-       apply tr_pi_intro; auto. 
-       apply tr_arrow_intro; auto.
-       change (var 1) with (@subst obj sh1 (var 0)). weaken Hp.
-       var_solv'.
-       simpl. change (nsucc (var 1)) with (@subst obj sh1 (nsucc (var 0))).
-       weaken Hp. apply nsucc_type. var_solv'.
-       simpsub_big. apply tr_pi_intro; auto.
-       apply tr_arrow_intro; auto.
-      { apply tr_equal_formation; auto.
-      weaken tr_booltp_formation.
-      apply eqapp_typed; auto; try apply nsucc_type; try var_solv'. constructor. }
-      { apply tr_equal_formation; auto; try apply nsucc_type; try var_solv'. }
-      simpsub_big. eapply (tr_compute_hyp _ [::]).
-      { constructor. apply equiv_equal. apply equiv_refl. apply eq_b_succ.
-        apply equiv_refl. }
-      (*split y into pair*)
-      simpl. rewrite make_app1. apply w_elim_hyp. weaken tr_booltp_formation.
-      weaken nat_U01.
-      change triv with (@subst obj (under 1 (dot (ppi2 (var 0))
-                                                 (dot (ppi1 (var 0)) sh1))) triv).
-      apply tr_sigma_eta_hyp.
-      simpsub_big. simpl. simpsub_big.
-      eapply (tr_compute_hyp _ [::]).
-      { constructor. apply equiv_equal. apply equiv_refl.
-        apply equiv_bite. apply reduce_equiv.
-        apply reduce_ppi1_beta. apply reduce_id. apply equiv_refl.
-        apply equiv_app. apply equiv_refl. apply equiv_app.
-        apply reduce_equiv. apply reduce_ppi2_beta. apply reduce_id.
-        apply equiv_refl. apply equiv_refl.
+    {
+      apply tr_pi_intro; auto. apply tr_arrow_intro; try weaken leq_type.
+      var_solv'.
+      apply nsucc_type; var_solv'. 
+      apply nsucc_type; var_solv'.
+      repeat apply nsucc_type; var_solv'.
+      simpsub. eapply tr_compute. 
+      eapply equiv_trans.
+      { try apply leq_succsucc_equiv; try apply equiv_refl. }
+      { apply equiv_app. apply equiv_app. apply equiv_refl.
+        apply reduce_equiv. apply reduce_app_beta; apply reduce_id. 
+        apply reduce_equiv. apply reduce_app_beta; apply reduce_id. 
       }
-      simpl. rewrite make_app2.
-      match goal with |- tr ?G (deq triv triv ?T) =>
-                      suffices: (tr G (oof (bite (var 2) triv triv) T)) end.
-      { intros Hannoying. constructor. eapply deq_intro. apply Hannoying. }
-      change triv with (@subst obj (under 2 sh1) triv).
-      apply tr_booltp_eta_hyp; simpl; simpsub_big.
-      { (*y' = 0*)
-        eapply (tr_compute_hyp _ [::]). { constructor. apply equiv_equal.
-        apply equiv_refl. apply reduce_equiv. apply reduce_bite_beta1.
-        apply reduce_id. apply equiv_refl. }
-        apply bool_contra. simpl. apply (deq_intro _#4 (var 0) (var 0)).
-        change (equal booltp bfalse btrue) with
-            (@subst obj (sh 1) (equal booltp bfalse btrue)). var_solv0. }
-      { (*y' = s y''*)
-       simpl.  eapply (tr_compute_hyp _ [::]).
-          { constructor. apply equiv_equal.
-        apply equiv_refl. apply reduce_equiv. apply reduce_bite_beta2.
-        apply reduce_id. apply equiv_refl. }
-          simpl. rewrite make_app1. eapply tr_compute_hyp.
-          { constructor. apply equiv_arrow. apply reduce_equiv.
-       apply reduce_bite_beta2.
-        apply reduce_id. apply equiv_refl. }
-          simpl.
-          constructor.
-          eapply (tr_transitivity _#2 (nsucc (app (var 1) triv))).
-          { (*succ x = succ (y' * *)
-            apply nsucc_type.
-            apply (deq_intro _#4 (app (app (var 2) (app (var 1) triv))
-                                      (var 0))
-                             (app (app (var 2) (app (var 1) triv))
-                                      (var 0))
-                  ).
-            apply (tr_arrow_elim _
-(equal booltp (app (eq_b (var 3)) (app (var 1) triv))
-       btrue)).
-      { apply tr_equal_formation; auto.
-      weaken tr_booltp_formation.
-      apply eqapp_typed; auto; try apply nsucc_type; try var_solv'.
-      apply (tr_arrow_elim _ unittp); auto.
+      apply equiv_refl. apply equiv_refl.
+      simpsub. simpl. 
       change 
-          (arrow unittp nattp) with (@subst obj (sh 2)
-(arrow unittp nattp)
-                                    ). var_solv'. constructor. constructor. }
-      {
-        apply tr_equal_formation; auto; try var_solv'.
-        apply (tr_arrow_elim _ unittp); auto.
-      change 
-          (arrow unittp nattp) with (@subst obj (sh 2)
-(arrow unittp nattp)
-                                    ). var_solv'. constructor. 
-      }
-      match goal with |- tr ?G (deq ?M ?M ?T) => change T with
-          (subst1 (app (var 1) triv)
-       (arrow
-          (equal booltp
-             (app (eq_b (var 4))
-                (var 0)) btrue)
-          (equal nattp (var 4) (var 0)))) end.
-      apply (tr_pi_elim _ nattp).
-      match goal with |- tr ?G (deq ?M ?M ?T) => change T with
-      ( subst (sh 3) (pi nattp
-          (arrow
-             (equal booltp
-                (app (eq_b (var 1)) (var 0)) btrue)
-             (equal nattp (var 1) (var 0))))) end. var_solv'.
-        apply (tr_arrow_elim _ unittp); auto.
-      change 
-          (arrow unittp nattp) with (@subst obj (sh 2)
-(arrow unittp nattp)
-                                    ). var_solv'. constructor.
-      match goal with |- tr ?G (deq ?M ?M ?T) => change T with
-          (subst (sh 1)
-       (equal booltp
-          (app (eq_b (var 2)) (app (var 0) triv))
-          btrue)) end. var_solv'. }
-          {  apply equal_succ.
-      change 
-          (arrow unittp nattp) with (@subst obj (sh 2)
-(arrow unittp nattp)
-                                    ). var_solv'.  } } } 
+       (app (app leqtp (var 1))
+            (nsucc (var 1))) with (subst sh1
+          (leq_t (var 0)
+             (nsucc (var 0)))
+                                  ). var_solv0.
+    } assumption.
 Qed.
-
-Lemma eqb_P G n m : tr G (oof n nattp) ->
-                    tr G (oof m nattp) ->
-  tr G (deq (app (eq_b n) m) btrue booltp) ->
-                    tr G (deq n m nattp).
-  intros.
-  match goal with |- tr G ?J => replace J with (substj (dot triv id)
-                                                    (deq (subst (sh 1) n)
-                                                         (subst (sh 1) m)
-                                                    nattp)
-                                             ) end.
-  2:{
-    unfold substj. simpsub. auto.
-  }
-  eapply tr_generalize. apply tr_equal_intro in H1. apply H1.
-  remember (subst (sh 1) n) as n'.
-  remember (subst (sh 1) m) as m'.
-  suffices: (tr (hyp_tm (equal booltp (app (eq_b n) m) btrue) :: G)
-                (deq triv (app (app (app eqb_sound_fn n') m') (var 0))
-                       (equal nattp n' m')
-            )).
-  move/ tr_eq_reflexivity => Hdeq.
-  constructor. assumption.
-  apply tr_symmetry. apply tr_equal_eta.
-  assert (tr
-    (hyp_tm (equal booltp (app (eq_b n) m) btrue)
-     :: G) (deq n' n' nattp)) as Hn. 
-    subst; change nattp with (@subst obj (sh 1) nattp);
-      rewrite ! subst_sh_shift; apply tr_weakening_append1; assumption.
-  assert (tr
-    (hyp_tm (equal booltp (app (eq_b n) m) btrue)
-     :: G) (deq m' m' nattp)) as Hm. 
-  subst; change nattp with (@subst obj (sh 1) nattp);
-      rewrite ! subst_sh_shift; apply tr_weakening_append1; assumption.
- (* replace (equal nattp n' m') with
-      (subst1 (var 0) (equal nattp (subst (sh 1) n') (subst (sh 1) m'))). *)
-  apply (tr_arrow_elim _ (equal booltp (app (eq_b n') m') btrue)
-        ).
-  - apply tr_equal_formation. weaken tr_booltp_formation.
-    apply eqapp_typed; assumption.
-    constructor. apply tr_equal_formation; auto.
-    - match goal with |- tr ?G (deq ?M ?M ?T) => replace T with  
-          (subst1 m' 
-       (arrow
-          (equal booltp (app (eq_b (subst (sh 1) n')) (var 0)) btrue)
-          (equal nattp (subst (sh 1) n') (var 0)))) end.
-      2:{
-        unfold subst1. simpsub_big.  auto.
-      }
-      apply (tr_pi_elim _ nattp).
-      match goal with |- tr ?G (deq ?M ?M ?T) => replace T with
-       (subst1 n' (pi nattp
-          (arrow
-             (equal booltp
-                (app
-                   (eq_b (var 1))
-                   (var 0)) btrue)
-             (equal nattp  (var 1)
-                (var 0))))) end.
-      apply (tr_pi_elim _ nattp); try assumption. apply eqb_sound.
-      simpsub_big. auto.
-      assumption.
-      match goal with |- tr ?G (deq ?M ?M ?T) => replace T with
-      (subst (sh 1) (equal booltp (app (eq_b n) m) btrue)) end. var_solv0.
-      subst. simpsub_big. auto.
-Qed.
-
